Tap

Discretion/Tactic/CategoryTheory/MonoidalComp.lean
@@ -45,97 +45,97 @@ A typeclass carrying a choice of monoidal structural isomorphism between two obj
 Used by the `⊗≫` monoidal composition operator, and the `coherence` tactic.
 -/
 -- We could likely turn this into a `Prop` valued existential if that proves useful.
-class MonoidalCoherence (X Y : C) where
+class MonoidalCoherence' (X Y : C) where
   /-- A monoidal structural isomorphism between two objects. -/
   iso : X ≅ Y
 
 /-- Notation for identities up to unitors and associators. -/
-scoped[CategoryTheory.MonoidalCategory] notation " ⊗𝟙 " =>
-  MonoidalCoherence.iso -- type as \ot 𝟙
+scoped[CategoryTheory.MonoidalCategory'] notation " ⊗𝟙 " =>
+  MonoidalCoherence'.iso -- type as \ot 𝟙
 
 /-- Construct an isomorphism between two objects in a monoidal category
 out of unitors and associators. -/
-abbrev monoidalIso (X Y : C) [MonoidalCoherence X Y] : X ≅ Y := MonoidalCoherence.iso
+abbrev monoidalIso' (X Y : C) [MonoidalCoherence' X Y] : X ≅ Y := MonoidalCoherence'.iso
 
 /-- Compose two morphisms in a monoidal category,
 inserting unitors and associators between as necessary. -/
-def monoidalComp {W X Y Z : C} [MonoidalCoherence X Y] (f : W ⟶ X) (g : Y ⟶ Z) : W ⟶ Z :=
+def monoidalComp' {W X Y Z : C} [MonoidalCoherence' X Y] (f : W ⟶ X) (g : Y ⟶ Z) : W ⟶ Z :=
   f ≫ ⊗𝟙.hom ≫ g
 
-@[inherit_doc monoidalComp]
-scoped[CategoryTheory.MonoidalCategory] infixr:80 " ⊗≫ " =>
-  monoidalComp -- type as \ot \gg
+@[inherit_doc monoidalComp']
+scoped[CategoryTheory.MonoidalCategory'] infixr:80 " ⊗≫ " =>
+  monoidalComp' -- type as \ot \gg
 
 /-- Compose two isomorphisms in a monoidal category,
 inserting unitors and associators between as necessary. -/
-def monoidalIsoComp {W X Y Z : C} [MonoidalCoherence X Y] (f : W ≅ X) (g : Y ≅ Z) : W ≅ Z :=
+def monoidalIsoComp' {W X Y Z : C} [MonoidalCoherence' X Y] (f : W ≅ X) (g : Y ≅ Z) : W ≅ Z :=
   f ≪≫ ⊗𝟙 ≪≫ g
 
-@[inherit_doc monoidalIsoComp]
-scoped[CategoryTheory.MonoidalCategory] infixr:80 " ≪⊗≫ " =>
-  monoidalIsoComp -- type as \ll \ot \gg
+@[inherit_doc monoidalIsoComp']
+scoped[CategoryTheory.MonoidalCategory'] infixr:80 " ≪⊗≫ " =>
+  monoidalIsoComp' -- type as \ll \ot \gg
 
-namespace MonoidalCoherence
+namespace MonoidalCoherence'
 
 variable [PremonoidalCategory C]
 
 @[simps]
-instance refl (X : C) : MonoidalCoherence X X := ⟨Iso.refl _⟩
+instance refl (X : C) : MonoidalCoherence' X X := ⟨Iso.refl _⟩
 
 @[simps]
-instance whiskerLeft (X Y Z : C) [MonoidalCoherence Y Z] :
-    MonoidalCoherence (X ⊗ Y) (X ⊗ Z) :=
+instance whiskerLeft (X Y Z : C) [MonoidalCoherence' Y Z] :
+    MonoidalCoherence' (X ⊗ Y) (X ⊗ Z) :=
   ⟨whiskerLeftIso X ⊗𝟙⟩
 
 @[simps]
-instance whiskerRight (X Y Z : C) [MonoidalCoherence X Y] :
-    MonoidalCoherence (X ⊗ Z) (Y ⊗ Z) :=
+instance whiskerRight (X Y Z : C) [MonoidalCoherence' X Y] :
+    MonoidalCoherence' (X ⊗ Z) (Y ⊗ Z) :=
   ⟨whiskerRightIso ⊗𝟙 Z⟩
 
 @[simps]
-instance tensor_right (X Y : C) [MonoidalCoherence (𝟙_ C) Y] :
-    MonoidalCoherence X (X ⊗ Y) :=
+instance tensor_right (X Y : C) [MonoidalCoherence' (𝟙_ C) Y] :
+    MonoidalCoherence' X (X ⊗ Y) :=
   ⟨(ρ_ X).symm ≪≫ (whiskerLeftIso X ⊗𝟙)⟩
 
 @[simps]
-instance tensor_right' (X Y : C) [MonoidalCoherence Y (𝟙_ C)] :
-    MonoidalCoherence (X ⊗ Y) X :=
+instance tensor_right' (X Y : C) [MonoidalCoherence' Y (𝟙_ C)] :
+    MonoidalCoherence' (X ⊗ Y) X :=
   ⟨whiskerLeftIso X ⊗𝟙 ≪≫ (ρ_ X)⟩
 
 @[simps]
-instance left (X Y : C) [MonoidalCoherence X Y] :
-    MonoidalCoherence (𝟙_ C ⊗ X) Y :=
+instance left (X Y : C) [MonoidalCoherence' X Y] :
+    MonoidalCoherence' (𝟙_ C ⊗ X) Y :=
   ⟨λ_ X ≪≫ ⊗𝟙⟩
 
 @[simps]
-instance left' (X Y : C) [MonoidalCoherence X Y] :
-    MonoidalCoherence X (𝟙_ C ⊗ Y) :=
+instance left' (X Y : C) [MonoidalCoherence' X Y] :
+    MonoidalCoherence' X (𝟙_ C ⊗ Y) :=
   ⟨⊗𝟙 ≪≫ (λ_ Y).symm⟩
 
 @[simps]
-instance right (X Y : C) [MonoidalCoherence X Y] :
-    MonoidalCoherence (X ⊗ 𝟙_ C) Y :=
+instance right (X Y : C) [MonoidalCoherence' X Y] :
+    MonoidalCoherence' (X ⊗ 𝟙_ C) Y :=
   ⟨ρ_ X ≪≫ ⊗𝟙⟩
 
 @[simps]
-instance right' (X Y : C) [MonoidalCoherence X Y] :
-    MonoidalCoherence X (Y ⊗ 𝟙_ C) :=
+instance right' (X Y : C) [MonoidalCoherence' X Y] :
+    MonoidalCoherence' X (Y ⊗ 𝟙_ C) :=
   ⟨⊗𝟙 ≪≫ (ρ_ Y).symm⟩
 
 @[simps]
-instance assoc (X Y Z W : C) [MonoidalCoherence (X ⊗ (Y ⊗ Z)) W] :
-    MonoidalCoherence ((X ⊗ Y) ⊗ Z) W :=
+instance assoc (X Y Z W : C) [MonoidalCoherence' (X ⊗ (Y ⊗ Z)) W] :
+    MonoidalCoherence' ((X ⊗ Y) ⊗ Z) W :=
   ⟨α_ X Y Z ≪≫ ⊗𝟙⟩
 
 @[simps]
-instance assoc' (W X Y Z : C) [MonoidalCoherence W (X ⊗ (Y ⊗ Z))] :
-    MonoidalCoherence W ((X ⊗ Y) ⊗ Z) :=
+instance assoc' (W X Y Z : C) [MonoidalCoherence' W (X ⊗ (Y ⊗ Z))] :
+    MonoidalCoherence' W ((X ⊗ Y) ⊗ Z) :=
   ⟨⊗𝟙 ≪≫ (α_ X Y Z).symm⟩
 
-end MonoidalCoherence
+end MonoidalCoherence'
 
-@[simp] lemma monoidalComp_refl {X Y Z : C} (f : X ⟶ Y) (g : Y ⟶ Z) :
+@[simp] lemma monoidalComp_refl' {X Y Z : C} (f : X ⟶ Y) (g : Y ⟶ Z) :
     f ⊗≫ g = f ≫ g := by
-  simp [monoidalComp]
+  simp [monoidalComp']
 
 end CategoryTheory
